src/Nomega.v
@@ -188,7 +188,7 @@ Definition within_bool (addr : N) (len : N) (a : N) : bool :=
   ((addr <=? a) && (a <? addr + len))%bool.
 
 Definition fits (addr1 len1 addr2 len2 : N) : Prop :=
-  within addr1 len1 addr2 /\ within addr1 len1 (addr2 + len2).
+  within addr1 len1 addr2 /\ addr2 + len2 <= addr1 + len1.
 
 Definition overlaps (addr len addr2 len2 : N) : Prop :=
   addr < addr2 + len2 /\ addr2 < addr + len.
@@ -391,8 +391,6 @@ Proof.
   nomega.
 Qed.
 
-(*** fits ***)
-
 (*** overlaps ***)
 
 Lemma overlaps_sym : forall addr1 len1 addr2 len2,
@@ -438,3 +436,8 @@ Proof.
   apply overlaps_within in H1; trivial;
   decisions; firstorder.
 Qed.
+
+(*** other theorems ***)
+
+Theorem Nlt_plus_1 : forall n : N, 0 < n + 1.
+Proof. nomega. Qed.
