src/ByteStringHeap.v
@@ -19,57 +19,6 @@ Require Import
 
 Generalizable All Variables.
 
-Theorem Nlt_plus_1 : forall n : N, 0 < n + 1.
-Proof. nomega. Qed.
-
-Corollary refine_computes_to_ret :
-  forall A f (v : A), f ↝ v <-> refine f (ret v).
-Proof.
-  split; intros.
-    apply refine_In.
-    exact H.
-  apply H.
-  constructor.
-Qed.
-
-Lemma refineEquiv_If_Then_Else_Bind :
-  forall (A B : Type) (i : bool) (t e : Comp A) (b : A -> Comp B),
-    refineEquiv (a <- If i Then t Else e; b a)
-                (If i Then a <- t; b a Else (a <- e; b a)).
-Proof. split; intros; destruct i; reflexivity. Qed.
-
-Theorem refine_If_Then_Else_bool :
-  forall (b : bool) A cpst cpse (res : Comp A),
-    (if b then refine cpst res else refine cpse res)
-      <-> refine (If b Then cpst Else cpse) res.
-Proof. split; intros; destruct b; auto. Qed.
-
-Global Program Instance refineEquiv_bind_dep : forall A (ca : Comp A) B,
-  Proper (forall_relation
-            (fun x0 : A =>
-               pointwise_relation (refine ca (ret x0)) refineEquiv) ==>
-            (@refineEquiv B))
-         (Bind_dep ca).
-Obligation 1.
-  intros ???.
-  split; intros; intros ??;
-  apply Bind_dep_inv in H0;
-  destruct H0;
-  exists x0;
-  destruct H0;
-  exists x1;
-  eapply H in c; eauto.
-Qed.
-
-Ltac destruct_computations :=
-  repeat match goal with
-  | [ H : _ ↝ _ |- _ ] => apply Bind_dep_inv in H; destruct H as [? [? H]]
-  | [ H : _ ↝ _ |- _ ] => apply Bind_inv in H; destruct H as [? [? H]]
-  | [ H : _ ↝ _ |- _ ] => apply Pick_inv in H
-  | [ H : _ ↝ _ |- _ ] => apply Return_inv in H; subst
-  (* | [ H : _ ↝ _ |- _ ] => destruct H *)
-  end.
-
 Module ByteStringHeap (Mem : Memory).
 
 Module Import BS := ByteString Mem.
@@ -121,61 +70,63 @@ Definition simply_widen_region (r : PS) : PS :=
    ; psOffset := psOffset r - 1
    ; psLength := psLength r + 1 |}.
 
-Lemma refine_local_memcpy (r : PS) :
-  0 < psLength r ->
-  fits (psBuffer r) (psBufLen r) (psBuffer r + 1) (psLength r) ->
-  (forall blk, Lookup (psBuffer r) blk (` (psHeap r))
-                 -> memSize blk = psBufLen r) ->
-  refineEquiv
-    (memcpy (` (psHeap r)) (psBuffer r) (psBuffer r + 1) (psLength r))
-    (blk <- { blk : MemoryBlock | Lookup (psBuffer r) blk (` (psHeap r)) };
-     ret (Update
-            (psBuffer r)
-            {| memSize := memSize blk
+Ltac competing_lookups R H A1 H0 A2 :=
+  let Heqe := fresh "Heqe" in
+  destruct (A1 =? A2) eqn:Heqe;
+    [ apply Neqb_ok in Heqe; subst;
+      pose proof (allocations_unique (proj2_sig R) _ _ H _ H0);
+      subst; try nomega
+    | apply N.eqb_neq in Heqe;
+      pose proof (allocations_no_overlap (proj2_sig R) _ H _ H0 Heqe);
+      try nomega ].
+
+Ltac resolve_contention :=
+  match goal with
+  | [ H : All _ ?R, H0 : Lookup ?A ?B ?R |- _ ] => destruct (H A B)
+  end.
+
+Lemma refine_local_memcpy (r : PS) data :
+  (0 < psLength r
+     -> fits (psBuffer r) (psBufLen r) (psBuffer r + 1) (psLength r)) ->
+  Lookup (psBuffer r) {| memSize := psBufLen r
+                       ; memData := data |} (` (psHeap r)) ->
+  refine
+    (ret (If 0 <? psLength r
+          Then Update (psBuffer r)
+            {| memSize := psBufLen r
              ; memData :=
-                 Union _ (KeepKeys (not ∘ within 1 (psLength r))
-                                   (memData blk))
+                 Union _ (KeepKeys (not ∘ within 1 (psLength r)) data)
                          (ShiftKeys 0 1 (KeepKeys (within 0 (psLength r))
-                                                  (memData blk))) |}
-            (` (psHeap r)), tt)).
+                                                  data)) |}
+            (` (psHeap r))
+          Else ` (psHeap r), tt))
+    (memcpy (` (psHeap r)) (psBuffer r) (psBuffer r + 1) (psLength r)).
 Proof.
-  unfold memcpy; split; intros.
-    intros ??.
-    apply Bind_inv in H2.
-    destruct H2 as [blk [H3 H4]].
-    apply Pick_inv in H3.
-    apply refine_computes_to_ret.
-    refine pick val (Some (psBuffer r, blk)).
-      simplify with monad laws.
-      refine pick val (Some (psBuffer r, blk)).
-        simplify with monad laws.
-        destruct H4.
-        do 4 f_equiv.
-        replace (psBuffer r - psBuffer r) with 0 by nomega.
-        replace (psBuffer r + 1 - psBuffer r) with 1 by nomega.
-        reflexivity.
-      intros; inv H2; intuition.
-      rewrite H1; auto.
-    intros; inv H2; intuition.
-    rewrite H1; auto.
-    nomega.
+  unfold memcpy; intros.
+  unfold IfDec_Then_Else; simpl.
   intros ??.
-  apply Bind_inv in H2.
-  destruct H2 as [[[n blk]|] [H3 H4]];
-  apply Pick_inv in H3;
-  [destruct (H3 n blk eq_refl) as [? [? ?]]; clear H3|];
-  apply refine_computes_to_ret.
-    refine pick val blk.
-      simplify with monad laws.
-      apply Bind_inv in H4.
-      destruct H4 as [[[n' blk']|] [H7 H8]].
-        apply Pick_inv in H7;
-        destruct (H7 n' blk' eq_refl) as [? [? ?]]; clear H7.
-        destruct H8.
-        admit.
-      clear H7.
-      destruct H8.
-Admitted.
+  destruct (0 <? psLength r) eqn:Heqe; simpl;
+  apply Bind_inv in H1;
+  destruct H1 as [blk1 [H1 H2]]; apply Pick_inv in H1;
+  destruct H2 as [blk2 [H2 H3]]; apply Pick_inv in H2;
+  destruct H3;
+  destruct blk1, blk2;
+  try destruct p;
+  try destruct p0;
+  try constructor;
+  try assert (H9 : 0 < psLength r) by nomega;
+  intuition.
+  - competing_lookups (psHeap r) H3 n H1 n0;
+    competing_lookups (psHeap r) H0 (psBuffer r) H1 n0.
+    replace (psBuffer r - psBuffer r) with 0 by nomega.
+    replace (psBuffer r + 1 - psBuffer r) with 1 by nomega.
+    constructor.
+  - competing_lookups (psHeap r) H0 (psBuffer r) H3 n.
+    resolve_contention; auto.
+  - competing_lookups (psHeap r) H0 (psBuffer r) H3 n.
+    resolve_contention; auto; nomega.
+  - resolve_contention; auto.
+Qed.
 
 Definition make_room_by_shifting_up (r : PS) : Comp PS :=
   res <- memcpy' (psHeap r) (psBuffer r) (psBuffer r + 1) (psLength r);
@@ -221,7 +172,7 @@ Definition ByteString_list_AbsR (or : Rep ByteStringSpec) (nr : PS) :=
   IF psBufLen nr = 0
   then psOffset nr = 0 /\ psLength nr = 0
   else
-    fits (psBuffer nr) (psBufLen nr + 1)
+    fits (psBuffer nr) (psBufLen nr)
          (psBuffer nr + psOffset nr) (psLength nr) /\
     exists data,
       Lookup (psBuffer nr) {| memSize := psBufLen nr; memData := data |}
@@ -280,15 +231,80 @@ Proof.
   rewrite refineEquiv_If_Then_Else_Bind in H.
   apply refine_If_Then_Else_bool in H.
   destruct (psLength r_n <? psBufLen r_n) eqn:Heqe2;
-  apply refine_computes_to_ret in H.
-  {
-    revert H.
-    unfold make_room_by_shifting_up, poke_at_offset.
-    autorewrite with monad laws; simpl.
-    rewrite N.add_0_r.
-    unfold memcpy', poke'.
-    rewrite refine_bind_dep_bind_ret; simpl.
-    setoid_rewrite refine_bind_dep_bind_ret; simpl.
+  apply refine_computes_to_ret in H;
+  revert H;
+  unfold make_room_by_shifting_up,
+         make_room_by_growing_buffer, poke_at_offset;
+  autorewrite with monad laws; simpl;
+  rewrite ?N.add_0_r;
+  unfold memcpy', realloc', poke';
+  rewrite refine_bind_dep_bind_ret; simpl;
+  setoid_rewrite refine_bind_dep_bind_ret;
+  simpl; intros;
+  apply Bind_dep_inv in H;
+  destruct H as [? [? ?]];
+  apply Bind_dep_inv in c;
+  destruct c as [? [? ?]]; destruct c;
+  destruct_AbsR AbsR; construct_AbsR;
+  try (right; split; [nomega|]; split; [nomega|]).
+  - eapply refine_local_memcpy in x1; eauto;
+    destruct (0 <? psLength r_n) eqn:Heqe;
+    try nomega; destruct x1, x3; simpl in *.
+      eexists.
+      split.
+        teardown.
+        exists {| memSize := psBufLen r_n
+                ; memData :=
+                    Union _ (KeepKeys (not ∘ within 1 (psLength r_n)) data)
+                            (ShiftKeys 0 1 (KeepKeys (within 0 (psLength r_n))
+                                                     data)) |}.
+        split.
+          decisions; f_equal; f_equal; nomega.
+        teardown.
+      intros; teardown.
+      destruct i using N.peano_ind.
+        left; nomega.
+      right; split; [nomega|]; clear IHi.
+      simpl; rewrite N2Nat.inj_succ in *; simpl.
+      rewrite H0 in H4; simpl in H4.
+      unfold KeepKeys, ShiftKeys; teardown.
+      destruct (within_dec 0 (N.succ (psLength r_n)) (N.succ i)).
+        right; teardown.
+        exists (i, x0); simpl.
+        split.
+          f_equal; nomega.
+        specialize (H4 _ _ H).
+        teardown; intuition.
+        nomega.
+      left; teardown.
+      split.
+        apply H4.
+        rewrite N2Nat.inj_succ, nth_overflow; trivial.
+        nomega.
+      unfold not, compose; intros.
+      contradiction n.
+      clear -H5.
+      destruct H5.
+      split; [nomega|]; simpl.
+      rewrite N.add_1_l in H0.
+      assumption.
+    eexists.
+    split.
+      teardown.
+      exists {| memSize := psBufLen r_n
+              ; memData := data |}.
+      split; auto.
+      decisions; f_equal; f_equal; nomega.
+    intros; teardown.
+    destruct i using N.peano_ind.
+      left; nomega.
+    right; split; [nomega|].
+    rewrite H0 in H4; simpl in H4; apply H4.
+    simpl; rewrite N2Nat.inj_succ in *; simpl.
+    destruct r_o; simpl in *; auto.
+    nomega.
+  - admit.
+  - admit.
 Admitted.
 
 Lemma refine_ret_eq_r : forall A (a b : A), refine (ret a) (ret b) -> a = b.
@@ -308,6 +324,12 @@ Proof.
   rewrite Nat.sub_0_r.
   reflexivity.
 Qed.
+
+Lemma it_fits : forall base size off len,
+  off + 1 < size ->
+  fits base size (base + off) len ->
+  fits base size (base + off + 1) (len - 1).
+Proof. nomega. Qed.
 
 Theorem buffer_uncons_sound : forall r_o r_n a,
   ByteString_list_AbsR r_o r_n
@@ -332,37 +354,38 @@ Proof.
   unfold peek'.
   rewrite refine_bind_dep_bind_ret; simpl.
   rewrite refine_bind_dep_ignore.
-  unfold peek.
-  autorewrite with monad laws; simpl.
-  intros.
+  unfold peek, FindBlockThatFits.
+  autorewrite with monad laws; simpl; intros.
   apply refine_computes_to_ret in H0.
-  apply Bind_inv in H0.
-  destruct H0, H0.
-  apply Return_inv in H1.
-  destruct a; tsubst; simpl in *.
-  apply Pick_inv in H0.
-  destruct H, H1.
-    nomega.
-  destruct H1, H1, H2.
-  assert (within (psBuffer r_n) (psBufLen r_n) (psBuffer r_n + psOffset r_n)).
-    nomega.
-  specialize (H0 _ _ H2 H4); simpl in *.
-  destruct r_o.
-    nomega.
-  split; simpl.
-    nomega.
-  destruct r_o.
-    left.
-    nomega.
-  right.
-  exists x0.
-  intuition.
-    nomega.
-  rewrite <- N.add_assoc.
-  apply H3.
-  rewrite N2Nat.inj_add.
-  apply H5.
-Qed.
+  destruct_computations.
+  destruct_AbsR H; construct_AbsR;
+  destruct x; try destruct p; simpl in *;
+  destruct r_o; simpl in *;
+  try nomega; right;
+  split; try nomega; split.
+  - rewrite N.add_assoc.
+    apply it_fits; trivial.
+    admit.
+  - eexists.
+    split.
+      exact H4.
+    intros.
+    rewrite <- N.add_assoc.
+    apply H5.
+    rewrite N.add_1_l, N2Nat.inj_succ.
+    assumption.
+  - rewrite N.add_assoc.
+    apply it_fits; trivial.
+    admit.
+  - eexists.
+    split.
+      exact H4.
+    intros.
+    rewrite <- N.add_assoc.
+    apply H5.
+    rewrite N.add_1_l, N2Nat.inj_succ.
+    assumption.
+Admitted.
 
 Theorem buffer_uncons_impl : forall r_o r_n a,
   ByteString_list_AbsR r_o r_n
